minmial

theories/SLFMinimal.v
@@ -14,27 +14,12 @@ License: CC-by 4.0.
 Set Implicit Arguments.
 From TLC Require Export LibCore.
 From Sep Require Export TLCbuffer Var Fmap.
-From Sep Require SepSimpl.
 
 
 (* ########################################################### *)
 (* ########################################################### *)
 (* ########################################################### *)
-(** * Imports *)
-
-(* ########################################################### *)
-(** ** Extensionality axioms *)
-
-(** These standard extensionality axioms come from TLC's LibAxiom.v file. *)
-
-Axiom functional_extensionality : forall A B (f g:A->B),
-  (forall x, f x = g x) ->
-  f = g.
-
-Axiom propositional_extensionality : forall (P Q:Prop),
-  (P <-> Q) ->
-  P = Q.
-
+(** * Source language *)
 
 (* ########################################################### *)
 (** ** Variables *)
@@ -58,11 +43,6 @@ Axiom propositional_extensionality : forall (P Q:Prop),
     associativity and commutativity. Without these two tactics, the
     proofs would be extremely tedious and fragile. *)
 
-
-(* ########################################################### *)
-(* ########################################################### *)
-(* ########################################################### *)
-(** * Source language *)
 
 (* ########################################################### *)
 (** ** Syntax *)
@@ -104,16 +84,21 @@ with trm : Type :=
   | trm_let : var -> trm -> trm -> trm
   | trm_if : trm -> trm -> trm -> trm.
 
-(** The state consists of a finite map from location to values.
+(** Coercions to improve conciseness in the statment of evaluation rules. *)
+
+Coercion val_bool : bool >-> val.
+Coercion val_int : Z >-> val.
+Coercion val_loc : loc >-> val.
+Coercion val_prim : prim >-> val.
+
+Coercion trm_val : val >-> trm.
+Coercion trm_var : var >-> trm.
+Coercion trm_app : trm >-> Funclass.
+
+(** A heap, a.k.a. state, consists of a finite map from location to values.
     Records and arrays are represented as sets of consecutive cells. *)
 
-Definition state : Type := fmap loc val.
-
-(** The type [heap], a.k.a. [state]. By convention, the "state"
-    refers to the full memory state, while the "heap" potentially
-    refers to only a fraction of the memory state. *)
-
-Definition heap : Type := state.
+Definition heap : Type := fmap loc val.
 
 
 (* ########################################################### *)
@@ -133,17 +118,16 @@ Implicit Types p : loc.
 Implicit Types n : int.
 Implicit Types v w r vf vx : val.
 Implicit Types t : trm.
-Implicit Types h : heap.
-Implicit Types s : state.
+Implicit Types s h : heap.
 
-(** The type of values is inhabited. *)
+(** The type of values is inhabited (useful for finite map operations). *)
 
 Global Instance Inhab_val : Inhab val.
 Proof using. apply (Inhab_of_val val_unit). Qed.
 
 
 (* ########################################################### *)
-(** ** Substitution *)
+(** ** Semantics *)
 
 (** Capture-avoiding substitution, standard definition. *)
 
@@ -158,25 +142,6 @@ Fixpoint subst (y:var) (w:val) (t:trm) : trm :=
   | trm_let x t1 t2 => trm_let x (aux t1) (if_y_eq x t2 (aux t2))
   | trm_if t0 t1 t2 => trm_if (aux t0) (aux t1) (aux t2)
   end.
-
-
-(* ########################################################### *)
-(** ** Coercions *)
-
-(** Coercions to improve conciseness in the statment of evaluation rules. *)
-
-Coercion val_bool : bool >-> val.
-Coercion val_int : Z >-> val.
-Coercion val_loc : loc >-> val.
-Coercion val_prim : prim >-> val.
-
-Coercion trm_val : val >-> trm.
-Coercion trm_var : var >-> trm.
-Coercion trm_app : trm >-> Funclass.
-
-
-(* ########################################################### *)
-(** ** Semantics *)
 
 (** Big-step evaluation judgement, written [eval s t s' v] *)
 
@@ -218,47 +183,33 @@ Inductive eval : heap -> trm -> heap -> val -> Prop :=
 (* ########################################################### *)
 (* ########################################################### *)
 (* ########################################################### *)
-(** * Heap predicates *)
-
-(** For technical reasons, to enable sharing the code implementing
-    the tactic [xmysimpl], we wrap the definitions inside a module. *)
-
-Module SepSimplArgs.
+(** * Heap predicates and entailment *)
 
 
 (* ########################################################### *)
-(** ** Hprop and entailment *)
+(** ** Extensionality axioms *)
+
+Axiom functional_extensionality : forall A B (f g:A->B),
+  (forall x, f x = g x) ->
+  f = g.
+
+Axiom propositional_extensionality : forall (P Q:Prop),
+  (P <-> Q) ->
+  P = Q.
+
+
+(* ########################################################### *)
+(** ** Core heap predicates *)
 
 (** The type of heap predicates is named [hprop]. *)
 
 Definition hprop := heap -> Prop.
-
-(** Entailment for heap predicates, written [H1 ==> H2]
-    (the entailment is linear, although our triples will be affine). *)
-
-Definition himpl (H1 H2:hprop) : Prop :=
-  forall h, H1 h -> H2 h.
-
-Notation "H1 ==> H2" := (himpl H1 H2) (at level 55) : hprop_scope.
-
-Open Scope hprop_scope.
-
-(** Entailment between postconditions, written [Q1 ===> Q2] *)
-
-Definition qimpl A (Q1 Q2:A->hprop) : Prop :=
-  forall (v:A), Q1 v ==> Q2 v.
-
-Notation "Q1 ===> Q2" := (qimpl Q1 Q2) (at level 55) : hprop_scope.
 
 (** Implicit types for meta-variables. *)
 
 Implicit Types P : Prop.
 Implicit Types H : hprop.
 Implicit Types Q : val->hprop.
-
-
-(* ########################################################### *)
-(** ** Definition of heap predicates *)
 
 (** Core heap predicates, and their associated notations:
 
@@ -269,8 +220,6 @@ Implicit Types Q : val->hprop.
     - [Q1 \*+ H2] denotes the separating conjunction extending a postcondition
     - [\exists x, H] denotes an existential
     - [\forall x, H] denotes a universal
-    - [H1 \-* H2] denotes a magic wand between heap predicates
-    - [Q1 \--* Q2] denotes a magic wand between postconditions
 
 *)
 
@@ -292,13 +241,22 @@ Definition hexists A (J:A->hprop) : hprop :=
 Definition hforall (A : Type) (J : A -> hprop) : hprop :=
   fun h => forall x, J x h.
 
+Definition hpure (P:Prop) : hprop := (* encoded as [\exists (p:P), \[]] *)
+  hexists (fun (p:P) => hempty).
+
 Notation "\[]" := (hempty)
   (at level 0) : hprop_scope.
+
+Notation "\[ P ]" := (hpure P)
+  (at level 0, format "\[ P ]") : hprop_scope.
 
 Notation "p '~~>' v" := (hsingle p v) (at level 32) : hprop_scope.
 
 Notation "H1 '\*' H2" := (hstar H1 H2)
   (at level 41, right associativity) : hprop_scope.
+
+Notation "Q \*+ H" := (fun x => hstar (Q x) H)
+  (at level 40) : hprop_scope.
 
 Notation "'\exists' x1 .. xn , H" :=
   (hexists (fun x1 => .. (hexists (fun xn => H)) ..))
@@ -310,40 +268,52 @@ Notation "'\forall' x1 .. xn , H" :=
   (at level 39, x1 binder, H at level 50, right associativity,
    format "'[' '\forall' '/ '  x1  ..  xn , '/ '  H ']'") : hprop_scope.
 
-(** Derived heap predicates.
-
-    The following operators are defined in terms of the ones
-    above, rather than as functions over heaps, to reduce the proof effort.
-    See the summary section in [SLFWand.v] for details. *)
-
-Definition hpure (P:Prop) : hprop :=
-  \exists (p:P), \[].
-
-Definition hwand (H1 H2 : hprop) : hprop :=
-  \exists H0, H0 \* hpure ((H0 \* H1) ==> H2).
-
-Definition qwand A (Q1 Q2:A->hprop) : hprop :=
-  \forall x, hwand (Q1 x) (Q2 x).
-
-Notation "\[ P ]" := (hpure P)
-  (at level 0, format "\[ P ]") : hprop_scope.
-
-Notation "Q \*+ H" := (fun x => hstar (Q x) H)
-  (at level 40) : hprop_scope.
-
-Notation "H1 \-* H2" := (hwand H1 H2)
-  (at level 43, right associativity) : hprop_scope.
-
-Notation "Q1 \--* Q2" := (qwand Q1 Q2)
-  (at level 43) : hprop_scope.
-
 
 
 (* ########################################################### *)
-(** ** Basic properties of Separation Logic operators *)
+(** ** Entailment *)
 
-(* ################################################ *)
-(** *** Tactic for automation *)
+(** Entailment for heap predicates, written [H1 ==> H2]
+    (the entailment is linear, although our triples will be affine). *)
+
+Definition himpl (H1 H2:hprop) : Prop :=
+  forall h, H1 h -> H2 h.
+
+Notation "H1 ==> H2" := (himpl H1 H2) (at level 55) : hprop_scope.
+
+Open Scope hprop_scope.
+
+(** Entailment between postconditions, written [Q1 ===> Q2] *)
+
+Definition qimpl A (Q1 Q2:A->hprop) : Prop :=
+  forall (v:A), Q1 v ==> Q2 v.
+
+Notation "Q1 ===> Q2" := (qimpl Q1 Q2) (at level 55) : hprop_scope.
+
+(** Entailment defines an order on heap predicates *)
+
+Lemma himpl_refl : forall H,
+  H ==> H.
+Proof using. introv M. auto. Qed.
+
+Lemma himpl_trans : forall H2 H1 H3,
+  (H1 ==> H2) ->
+  (H2 ==> H3) ->
+  (H1 ==> H3).
+Proof using. introv M1 M2. unfolds* himpl. Qed.
+
+Lemma himpl_antisym : forall H1 H2,
+  (H1 ==> H2) ->
+  (H2 ==> H1) ->
+  (H1 = H2).
+Proof using. introv M1 M2. applys pred_ext_1. intros h. iff*. Qed.
+
+Hint Resolve himpl_refl.
+Hint Unfold qimpl.
+
+
+(* ########################################################### *)
+(** ** Minimal automation for heap disjointness *)
 
 (** [auto] is set up to process goals of the form [h1 = h2] by calling
     [fmap_eq], which proves equality modulo associativity and commutativity. *)
@@ -363,79 +333,25 @@ Tactic Notation "fmap_disjoint_pre" :=
 Hint Extern 1 (Fmap.disjoint _ _) => fmap_disjoint_pre.
 
 
-(* ################################################ *)
-(** *** Properties of [himpl] and [qimpl] *)
+(* ########################################################### *)
+(** ** Properties of [hstar] *)
 
-Lemma himpl_refl : forall H,
-  H ==> H.
-Proof using. introv M. auto. Qed.
-
-Hint Resolve himpl_refl.
-
-Lemma himpl_trans : forall H2 H1 H3,
-  (H1 ==> H2) ->
-  (H2 ==> H3) ->
-  (H1 ==> H3).
-Proof using. introv M1 M2. unfolds* himpl. Qed.
-
-Lemma himpl_trans_r : forall H2 H1 H3,
-   H2 ==> H3 ->
-   H1 ==> H2 ->
-   H1 ==> H3.
-Proof using. introv M1 M2. applys* himpl_trans M2 M1. Qed.
-
-Lemma himpl_antisym : forall H1 H2,
-  (H1 ==> H2) ->
-  (H2 ==> H1) ->
-  (H1 = H2).
-Proof using. introv M1 M2. applys pred_ext_1. intros h. iff*. Qed.
-
-Lemma hprop_op_comm : forall (op:hprop->hprop->hprop),
-  (forall H1 H2, op H1 H2 ==> op H2 H1) ->
-  (forall H1 H2, op H1 H2 = op H2 H1).
-Proof using. introv M. intros. applys himpl_antisym; applys M. Qed.
-
-Lemma qimpl_refl : forall A (Q:A->hprop),
-  Q ===> Q.
-Proof using. intros. unfolds*. Qed.
-
-Hint Resolve qimpl_refl.
-
-
-(* ################################################ *)
-(** *** Properties of [hempty] *)
-
-Lemma hempty_intro :
-  \[] heap_empty.
-Proof using. unfolds*. Qed.
-
-Lemma hempty_inv : forall h,
-  \[] h ->
-  h = heap_empty.
-Proof using. auto. Qed.
-
-
-(* ################################################ *)
-(** *** Properties of [hstar] *)
-
+(* Internal lemma: useful to unfold the definition of [hstar] *)
 Lemma hstar_intro : forall H1 H2 h1 h2,
   H1 h1 ->
   H2 h2 ->
   Fmap.disjoint h1 h2 ->
   (H1 \* H2) (Fmap.union h1 h2).
-Proof using. intros. exists~ h1 h2. Qed.
-
-Lemma hstar_inv : forall H1 H2 h,
-  (H1 \* H2) h ->
-  exists h1 h2, H1 h1 /\ H2 h2 /\ Fmap.disjoint h1 h2 /\ h = Fmap.union h1 h2.
-Proof using. introv M. applys M. Qed.
+Proof using. intros. exists* h1 h2. Qed.
 
 Lemma hstar_comm : forall H1 H2,
    H1 \* H2 = H2 \* H1.
 Proof using.
-  applys hprop_op_comm. unfold hprop, hstar. intros H1 H2.
-  intros h (h1&h2&M1&M2&D&U). rewrite~ Fmap.union_comm_of_disjoint in U.
-  exists* h2 h1.
+  unfold hprop, hstar. intros H1 H2. applys himpl_antisym.
+  { intros h (h1&h2&M1&M2&D&U). 
+    rewrite* Fmap.union_comm_of_disjoint in U. exists* h2 h1. }
+  { intros h (h1&h2&M1&M2&D&U). 
+    rewrite* Fmap.union_comm_of_disjoint in U. exists* h2 h1. }
 Qed.
 
 Lemma hstar_assoc : forall H1 H2 H3,
@@ -443,38 +359,31 @@ Lemma hstar_assoc : forall H1 H2 H3,
 Proof using.
   intros H1 H2 H3. applys himpl_antisym; intros h.
   { intros (h'&h3&(h1&h2&M3&M4&D'&U')&M2&D&U). subst h'.
-    exists h1 (h2 \+ h3). splits~. { applys* hstar_intro. } }
+    exists h1 (h2 \+ h3). splits*. { applys* hstar_intro. } }
   { intros (h1&h'&M1&(h2&h3&M3&M4&D'&U')&D&U). subst h'.
-    exists (h1 \+ h2) h3. splits~. { applys* hstar_intro. } }
+    exists (h1 \+ h2) h3. splits*. { applys* hstar_intro. } }
 Qed.
 
 Lemma hstar_hempty_l : forall H,
   \[] \* H = H.
 Proof using.
   intros. applys himpl_antisym; intros h.
-  { intros (h1&h2&M1&M2&D&U). forwards E: hempty_inv M1. subst.
-    rewrite~ Fmap.union_empty_l. }
-  { intros M. exists heap_empty h. splits~. { applys hempty_intro. } }
-Qed.
-
-Lemma hstar_hempty_r : forall H,
-  H \* \[] = H.
-Proof using.
-  applys neutral_r_of_comm_neutral_l. applys~ hstar_comm. applys~ hstar_hempty_l.
+  { intros (h1&h2&M1&M2&D&U). hnf in M1. subst. rewrite* Fmap.union_empty_l. }
+  { intros M. exists heap_empty h. splits*. { hnf. auto. } }
 Qed.
 
 Lemma hstar_hexists : forall A (J:A->hprop) H,
   (hexists J) \* H = hexists (fun x => (J x) \* H).
 Proof using.
   intros. applys himpl_antisym; intros h.
-  { intros (h1&h2&(x&M1)&M2&D&U). exists~ x h1 h2. }
-  { intros (x&(h1&h2&M1&M2&D&U)). exists h1 h2. splits~. { exists~ x. } }
+  { intros (h1&h2&(x&M1)&M2&D&U). exists* x h1 h2. }
+  { intros (x&(h1&h2&M1&M2&D&U)). exists h1 h2. splits~. { exists* x. } }
 Qed.
 
 Lemma hstar_hforall : forall H A (J:A->hprop),
   (hforall J) \* H ==> hforall (J \*+ H).
 Proof using.
-  intros. intros h M. destruct M as (h1&h2&M1&M2&D&U). intros x. exists~ h1 h2.
+  intros. intros h M. destruct M as (h1&h2&M1&M2&D&U). intros x. exists* h1 h2.
 Qed.
 
 Lemma himpl_frame_l : forall H2 H1 H1',
@@ -482,51 +391,26 @@ Lemma himpl_frame_l : forall H2 H1 H1',
   (H1 \* H2) ==> (H1' \* H2).
 Proof using. introv W (h1&h2&?). exists* h1 h2. Qed.
 
+(** Additional, symmetric results *)
+ 
+Lemma hstar_hempty_r : forall H,
+  H \* \[] = H.
+Proof using.
+  applys neutral_r_of_comm_neutral_l. applys* hstar_comm. applys* hstar_hempty_l.
+Qed.
+
 Lemma himpl_frame_r : forall H1 H2 H2',
   H2 ==> H2' ->
   (H1 \* H2) ==> (H1 \* H2').
 Proof using.
-  introv M. do 2 rewrite (@hstar_comm H1). applys~ himpl_frame_l.
-Qed.
-
-Lemma himpl_frame_lr : forall H1 H1' H2 H2',
-  H1 ==> H1' ->
-  H2 ==> H2' ->
-  (H1 \* H2) ==> (H1' \* H2').
-Proof using.
-  introv M1 M2. applys himpl_trans. applys~ himpl_frame_l M1. applys~ himpl_frame_r.
-Qed.
-
-Lemma himpl_hstar_trans_l : forall H1 H2 H3 H4,
-  H1 ==> H2 ->
-  H2 \* H3 ==> H4 ->
-  H1 \* H3 ==> H4.
-Proof using.
-  introv M1 M2. applys himpl_trans M2. applys himpl_frame_l M1.
-Qed.
-
-Lemma himpl_hstar_trans_r : forall H1 H2 H3 H4,
-  H1 ==> H2 ->
-  H3 \* H2 ==> H4 ->
-  H3 \* H1 ==> H4.
-Proof using.
-  introv M1 M2. applys himpl_trans M2. applys himpl_frame_r M1.
+  introv M. do 2 rewrite (@hstar_comm H1). applys* himpl_frame_l.
 Qed.
 
 
 (* ################################################ *)
-(** ***  Properties of [hpure] *)
+(** *** Properties of [hpure] *)
 
-Lemma hpure_intro : forall P,
-  P ->
-  \[P] heap_empty.
-Proof using. introv M. exists M. unfolds*. Qed.
-
-Lemma hpure_inv : forall P h,
-  \[P] h ->
-  P /\ h = heap_empty.
-Proof using. introv (p&M). split~. Qed.
-
+(* Internal lemma, useful for proofs *)
 Lemma hstar_hpure : forall P H h,
   (\[P] \* H) h = (P /\ H h).
 Proof using.
@@ -541,47 +425,11 @@ Lemma himpl_hstar_hpure_r : forall P H H',
   H ==> (\[P] \* H').
 Proof using. introv HP W. intros h K. rewrite* hstar_hpure. Qed.
 
-Lemma hpure_inv_hempty : forall P h,
-  \[P] h ->
-  P /\ \[] h.
-Proof using.
-  introv M. rewrite <- hstar_hpure. rewrite~ hstar_hempty_r.
-Qed.
-
-Lemma hpure_intro_hempty : forall P h,
-  \[] h ->
-  P ->
-  \[P] h.
-Proof using.
-  introv M N. rewrite <- (hstar_hempty_l \[P]).
-  rewrite hstar_comm. rewrite~ hstar_hpure.
-Qed.
-
-Lemma himpl_hempty_hpure : forall P,
-  P ->
-  \[] ==> \[P].
-Proof using. introv HP. intros h Hh. applys* hpure_intro_hempty. Qed.
-
 Lemma himpl_hstar_hpure_l : forall P H H',
   (P -> H ==> H') ->
   (\[P] \* H) ==> H'.
 Proof using.
   introv W Hh. rewrite hstar_hpure in Hh. applys* W.
-Qed.
-
-Lemma hempty_eq_hpure_true :
-  \[] = \[True].
-Proof using.
-  applys himpl_antisym; intros h M.
-  { applys* hpure_intro_hempty. }
-  { forwards*: hpure_inv_hempty M. }
-Qed.
-
-Lemma hfalse_hstar_any : forall H,
-  \[False] \* H = \[False].
-Proof using.
-  intros. applys himpl_antisym; intros h; rewrite hstar_hpure; intros M.
-  { false*. } { lets: hpure_inv_hempty M. false*. }
 Qed.
 
 
@@ -596,7 +444,7 @@ Proof using. introv W. intros h (x&Hh). applys* W. Qed.
 Lemma himpl_hexists_r : forall A (x:A) H J,
   (H ==> J x) ->
   H ==> (hexists J).
-Proof using. introv W. intros h. exists x. apply~ W. Qed.
+Proof using. introv W. intros h. exists x. apply* W. Qed.
 
 Lemma himpl_hexists : forall A (J1 J2:A->hprop),
   J1 ===> J2 ->
@@ -612,12 +460,12 @@ Qed.
 Lemma himpl_hforall_r : forall A (J:A->hprop) H,
   (forall x, H ==> J x) ->
   H ==> (hforall J).
-Proof using. introv M. intros h Hh x. apply~ M. Qed.
+Proof using. introv M. intros h Hh x. apply* M. Qed.
 
 Lemma himpl_hforall_l : forall A x (J:A->hprop) H,
   (J x ==> H) ->
   (hforall J) ==> H.
-Proof using. introv M. intros h Hh. apply~ M. Qed.
+Proof using. introv M. intros h Hh. apply* M. Qed.
 
 Lemma himpl_hforall : forall A (J1 J2:A->hprop),
   J1 ===> J2 ->
@@ -628,134 +476,13 @@ Qed.
 
 
 (* ################################################ *)
-(** *** Properties of [hwand] *)
-
-Lemma hwand_equiv : forall H0 H1 H2,
-  (H0 ==> H1 \-* H2) <-> (H0 \* H1 ==> H2).
-Proof using.
-  unfold hwand. iff M.
-  { applys himpl_hstar_trans_l (rm M).
-    rewrite hstar_hexists. applys himpl_hexists_l. intros H.
-    rewrite (hstar_comm H). rewrite hstar_assoc.
-    applys~ himpl_hstar_hpure_l. }
-  { applys himpl_hexists_r H0.
-    rewrite <- (hstar_hempty_r H0) at 1.
-    applys himpl_frame_r. applys himpl_hempty_hpure M. }
-Qed.
-
-Lemma himpl_hwand_r : forall H1 H2 H3,
-  H1 \* H2 ==> H3 ->
-  H1 ==> (H2 \-* H3).
-Proof using. introv M. rewrite~ hwand_equiv. Qed.
-
-Lemma himpl_hwand_r_inv : forall H1 H2 H3,
-  H1 ==> (H2 \-* H3) ->
-  H1 \* H2 ==> H3.
-Proof using. introv M. rewrite~ <- hwand_equiv. Qed.
-
-Lemma hwand_cancel : forall H1 H2,
-  H1 \* (H1 \-* H2) ==> H2.
-Proof using. intros. rewrite hstar_comm. rewrite~ <- hwand_equiv. Qed.
-
-Arguments hwand_cancel : clear implicits.
-
-Lemma himpl_hempty_hwand_same : forall H,
-  \[] ==> (H \-* H).
-Proof using. intros. rewrite hwand_equiv. rewrite~ hstar_hempty_l. Qed.
-
-Lemma hwand_hempty_l : forall H,
-  (\[] \-* H) = H.
-Proof using.
-  intros. applys himpl_antisym.
-  { rewrite <- hstar_hempty_l at 1. applys hwand_cancel. }
-  { rewrite hwand_equiv. rewrite~ hstar_hempty_r. }
-Qed.
-
-Lemma hwand_hpure_l_intro : forall (P:Prop) H,
-  P ->
-  \[P] \-* H ==> H.
-Proof using.
-  introv HP. rewrite <- hstar_hempty_l at 1.
-  forwards~ K: himpl_hempty_hpure P.
-  applys himpl_hstar_trans_l K. applys hwand_cancel.
-Qed.
-
-Arguments hwand_hpure_l_intro : clear implicits.
-
-Lemma hwand_curry : forall H1 H2 H3,
-  (H1 \* H2) \-* H3 ==> H1 \-* (H2 \-* H3).
-Proof using.
-  intros. do 2 rewrite hwand_equiv.
-  rewrite hstar_assoc. rewrite hstar_comm. applys hwand_cancel.
-Qed.
-
-Lemma hwand_uncurry : forall H1 H2 H3,
-  H1 \-* (H2 \-* H3) ==> (H1 \* H2) \-* H3.
-Proof using.
-  intros. rewrite hwand_equiv. rewrite <- (hstar_comm (H1 \* H2)).
-  rewrite (@hstar_comm H1). rewrite hstar_assoc.
-  applys himpl_hstar_trans_r.
-  { applys hwand_cancel. } { applys hwand_cancel. }
-Qed.
-
-Lemma hwand_curry_eq : forall H1 H2 H3,
-  (H1 \* H2) \-* H3 = H1 \-* (H2 \-* H3).
-Proof using.
-  intros. applys himpl_antisym.
-  { applys hwand_curry. }
-  { applys hwand_uncurry. }
-Qed.
-
-
-(* ################################################ *)
-(** *** Properties of qwand *)
-
-Lemma qwand_equiv : forall H A (Q1 Q2:A->hprop),
-  H ==> (Q1 \--* Q2) <-> (Q1 \*+ H) ===> Q2.
-Proof using.
-  unfold qwand. iff M.
-  { intros x. rewrite hstar_comm. applys himpl_hstar_trans_l (rm M).
-    applys himpl_trans. applys hstar_hforall. simpl.
-    applys himpl_hforall_l x. rewrite hstar_comm. applys hwand_cancel. }
-  { applys himpl_hforall_r. intros x. rewrite hwand_equiv. rewrite* hstar_comm. }
-Qed.
-
-Lemma qwand_cancel : forall A (Q1 Q2:A->hprop),
-  Q1 \*+ (Q1 \--* Q2) ===> Q2.
-Proof using. intros. rewrite <- qwand_equiv. applys qimpl_refl. Qed.
-
-Lemma himpl_qwand_r : forall A (Q1 Q2:A->hprop) H,
-  Q1 \*+ H ===> Q2 ->
-  H ==> (Q1 \--* Q2).
-Proof using. introv M. rewrite~ qwand_equiv. Qed.
-
-Arguments himpl_qwand_r [A].
-
-Lemma qwand_specialize : forall A (x:A) (Q1 Q2:A->hprop),
-  (Q1 \--* Q2) ==> (Q1 x \-* Q2 x).
-Proof using. intros. applys* himpl_hforall_l x. Qed.
-
-Arguments qwand_specialize [ A ].
-
-
-(* ################################################ *)
 (** *** Properties of [hsingle] *)
-
-Lemma hsingle_intro : forall p v,
-  p <> null ->
-  (p ~~> v) (Fmap.single p v).
-Proof using. introv N. hnfs*. Qed.
-
-Lemma hsingle_inv: forall p v h,
-  (p ~~> v) h ->
-  h = Fmap.single p v /\ p <> null.
-Proof using. auto. Qed.
 
 Lemma hsingle_not_null : forall p v,
   (p ~~> v) ==> (p ~~> v) \* \[p <> null].
 Proof using.
   introv. intros h (K&N). rewrite hstar_comm, hstar_hpure.
-  split*. subst. applys* hsingle_intro.
+  split*. subst. hnfs*.
 Qed.
 
 Lemma hstar_hsingle_same_loc : forall p v1 v2,
@@ -765,226 +492,50 @@ Proof using.
   subst. applys* Fmap.disjoint_single_single_same_inv.
 Qed.
 
-Arguments hstar_hsingle_same_loc : clear implicits.
-
 
 (* ########################################################### *)
-(** ** The [xsimpl] tactic *)
+(** * Minimal tactics for simplifying and rewriting entailments *)
 
-(** The definitions and properties above enable us to instantiate
-    the [xsimpl] tactic, which implements powerful simplifications
-    for Separation Logic entailments.
+(** [xsimpl] simplifies an entailment in simple cases. *)
 
-    For technical reasons, we need to provide a definition for [hgc],
-    a restriction of [htop] to affine heap predicates. For our purpose,
-    it suffices to define [hgc] as an alias for [htop]. *)
+Hint Rewrite hstar_assoc hstar_hempty_l hstar_hempty_r : hstar.
 
-
-(* ################################################ *)
-(** *** Definition and properties of [haffine] and [hgc] *)
-
-Definition haffine (H:hprop) :=
-  True.
-
-Lemma haffine_hany : forall (H:hprop),
-  haffine H.
-Proof using. unfold haffine. auto. Qed.
-
-Lemma haffine_hempty :
-  haffine \[].
-Proof using. applys haffine_hany. Qed.
-
-Definition hgc := (* equivalent to [\exists H, \[haffine H] \* H] *)
-  \exists H, H.
-
-Definition htop := hgc.
-
-Notation "\GC" := (hgc) : hprop_scope.
-
-Lemma haffine_hgc :
-  haffine \GC.
-Proof using. applys haffine_hany. Qed.
-
-Lemma himpl_hgc_r : forall H,
-  haffine H ->
-  H ==> \GC.
-Proof using. introv M. Admitted.
-
-Lemma hstar_hgc_hgc :
-  \GC \* \GC = \GC.
-Proof using. Admitted.
-
-
-(* ################################################ *)
-(** *** Functor instantiation to obtain [xsimpl] *)
-
-Notation "\Top" := (htop) : hprop_scope.
-
-Lemma htop_intro : forall h,
-  \Top h.
-Proof using. intros. exists~ (=h). Qed.
-
-Lemma himpl_htop_r : forall H,
-  H ==> \Top.
-Proof using. intros. intros h Hh. applys* htop_intro. Qed.
-
-Lemma htop_eq :
-  \Top = (\exists H, H).
-Proof using. auto. Qed.
-
-Lemma hstar_htop_htop :
-  \Top \* \Top = \Top.
-Proof using.
-  applys himpl_antisym.
-  { applys himpl_htop_r. }
-  { rewrite <- hstar_hempty_r at 1. applys himpl_frame_r. applys himpl_htop_r. }
-Qed.
-
-
-End SepSimplArgs.
-
-
-(** We are now ready to instantiate the functor, and open the
-    contents of the module [SepHsimplArgs], essentially pretending
-    that we inlined here its contents. *)
-
-Module Export HS := SepSimpl.XsimplSetup(SepSimplArgs).
-
-Export SepSimplArgs.
-
-(** At this point, the tactic [xsimpl] is defined.
-    There remains to customize the tactic so that it recognizes
-    the predicate [p ~~> v] in a special way when performing
-    simplifications. *)
-
-(*  Internal hack: (the comment only makes sense in the context of [SepSimpl]).
-    [xsimpl_pick_hsingle H] applies to a goal of the form
-    [Xsimpl (Hla, Hlw, Hlt) HR], where [Hla] is of the form
-    [H1 \* .. \* Hn \* \[]], and where [H] is of the form [p ~~> v]
-    It searches for [p ~~> v'] among the [Hi]. If it finds it, it
-    moves this [Hi] to the front, just before [H1]. Else, it fails. *)
-
-Ltac xsimpl_pick_hsingle H :=
-  match H with hsingle ?p ?v =>
-    xsimpl_pick_st ltac:(fun H' =>
-      match H' with (hsingle p ?v') =>
-        constr:(true) end)
+Ltac xsimpl_core :=
+  try match goal with |- _ ===> _ => intros ? end;
+  autorewrite with hstar;
+  repeat match goal with
+  | |- ?H \* _ ==> ?H \* _ => apply himpl_frame_r
+  | |- _ \* ?H ==> _ \* ?H => apply himpl_frame_l
+  | |- _ \* ?H ==> ?H \* _ => rewrite hstar_comm; apply himpl_frame_r
+  | |- ?H \* _ ==> _ \* ?H => rewrite hstar_comm; apply himpl_frame_l
+  | |- ?H ==> ?H => apply himpl_refl 
+  | |- ?H ==> ?H' => is_evar H'; apply himpl_refl 
   end.
 
-(** Internal hack:
-    The following instantiation of the [xsimpl] hook enables the tactic
-    to simplify [p ~~> v] against [p ~~> v'] by generating the
-    side-condition [v = v']. *)
+Tactic Notation "xsimpl" := xsimpl_core.
+Tactic Notation "xsimpl" "*" := xsimpl; auto_star.
 
-Ltac xsimpl_hook H ::=
-  match H with
-  | hsingle _ _ => xsimpl_pick_hsingle H; apply xsimpl_lr_cancel_eq;
-                   [ xsimpl_lr_cancel_eq_repr_post tt | ]
-  end.
+(** [xchange] helps rewriting in entailments. *)
 
-(** At this point, the tactic [xsimpl] is available.
-    See the file [SLFHimpl.v] for demos of its usage. *)
-
-(** One last hack is to improve the [math] tactic so that it is able
-    to handle the [val_int] coercion in goals and hypotheses of the
-     form [val_int ?n = val_int ?m], and so that it is able to process
-     the well-founded relations [dowto] and [upto] for induction on
-     integers. *)
-
-Ltac math_0 ::=
-  unfolds downto, upto;
-  try match goal with
-  | |- val_int _ = val_int _ => fequal
-  | H: val_int _ = val_int _ |- _ => inverts H
-  end.
-
-(** From now on, all operators have opaque definitions *)
-
-Global Opaque hempty hpure hstar hsingle hexists hforall
-              hwand qwand htop hgc haffine.
-
-
-
-(* ########################################################### *)
-(* ########################################################### *)
-(* ########################################################### *)
-(** * Reasoning rules *)
-
-
-Ltac xmysimpl_core :=
-  try match goal with |- _ = _ :> val -> hprop => intros ? end;
-  repeat rewrite hstar_assoc;
-  repeat first [ apply himpl_frame_r
-               | apply himpl_frame_l 
-               | match goal with |- ?H = ?H => apply himpl_refl end ].
-
-Tactic Notation "xmysimpl" := xmysimpl_core.
-
-Tactic Notation "xmysimpl" "*" := xmysimpl; auto_star.
-
-
-(* ########################################################### *)
-(** ** Evaluation rules for primitives in Separation style *)
-
-(** These lemmas reformulated the big-step evaluation rule
-    in a Separation-Logic friendly presentation, that is,
-    by using disjoint unions as much as possible.
-    It is not needed to follow through these proofs. *)
-
-Lemma eval_ref_sep : forall s1 s2 v p,
-  s2 = Fmap.single p v ->
-  Fmap.disjoint s2 s1 ->
-  eval s1 (val_ref v) (Fmap.union s2 s1) (val_loc p).
+Lemma xchange_lemma : forall H1 H1',
+  H1 ==> H1' -> forall H H' H2,
+  H ==> H1 \* H2 ->
+  H1' \* H2 ==> H' ->
+  H ==> H'.
 Proof using.
-  introv -> D. forwards Dv: Fmap.indom_single p v.
-  rewrite <- Fmap.update_eq_union_single. applys~ eval_ref.
-  { intros N. applys~ Fmap.disjoint_inv_not_indom_both D N. }
+  introv M1 M2 M3. applys himpl_trans M2. applys himpl_trans M3.
+  applys himpl_frame_l. applys M1.
 Qed.
 
-Lemma eval_get_sep : forall s s2 p v,
-  s = Fmap.union (Fmap.single p v) s2 ->
-  eval s (val_get (val_loc p)) s v.
-Proof using.
-  introv ->. forwards Dv: Fmap.indom_single p v.
-  applys_eq eval_get 1.
-  { applys~ Fmap.indom_union_l. }
-  { rewrite~ Fmap.read_union_l. rewrite~ Fmap.read_single. }
-Qed.
+Ltac xchange_core M :=
+  forwards_nounfold_then M ltac:(fun K =>
+    eapply xchange_lemma; [ eapply K | xsimpl | ]).
 
-Lemma eval_set_sep : forall s1 s2 h2 p v1 v2,
-  s1 = Fmap.union (Fmap.single p v1) h2 ->
-  s2 = Fmap.union (Fmap.single p v2) h2 ->
-  Fmap.disjoint (Fmap.single p v1) h2 ->
-  eval s1 (val_set (val_loc p) v2) s2 val_unit.
-Proof using.
-  introv -> -> D. forwards Dv: Fmap.indom_single p v1.
-  applys_eq eval_set 2.
-  { applys~ Fmap.indom_union_l. }
-  { rewrite~ Fmap.update_union_l. fequals.
-    rewrite~ Fmap.update_single. }
-Qed.
+Tactic Notation "xchange" constr(M) := xchange_core M.
 
-Lemma eval_free_sep : forall s1 s2 v p,
-  s1 = Fmap.union (Fmap.single p v) s2 ->
-  Fmap.disjoint (Fmap.single p v) s2 ->
-  eval s1 (val_free p) s2 val_unit.
-Proof using.
-  introv -> D. forwards Dv: Fmap.indom_single p v.
-  applys_eq eval_free 2.
-  { applys~ Fmap.indom_union_l. }
-  { rewrite~ Fmap.remove_union_single_l.
-    intros Dl. applys Fmap.disjoint_inv_not_indom_both D Dl.
-    applys Fmap.indom_single. }
-Qed.
-
-
-(* ########################################################### *)
-(** ** Tactic himpl-fold *)
-
-(** The tactic [himpl_fold] applies to a goal of the form [H1 h].
-    It searches the context for an assumption of the from [H2 h],
-    then replaces the goal with [H1 ==> H2].
-    It also deletes the assumption [H2 h]. *)
+(** [himpl_fold] applies to a goal of the form [H1 h]. It searches the
+    context for an assumption of the from [H2 h], then replaces the goal
+    with [H1 ==> H2], and deletes the assumption [H2 h]. *)
 
 Lemma himpl_inv : forall H1 H2 h,
   (H1 ==> H2) ->
@@ -997,8 +548,58 @@ Ltac himpl_fold_core tt :=
     applys himpl_inv N; clear N end.
 
 Tactic Notation "himpl_fold" := himpl_fold_core tt.
-Tactic Notation "himpl_fold" "~" := himpl_fold; auto_tilde.
 Tactic Notation "himpl_fold" "*" := himpl_fold; auto_star.
+
+
+(* ########################################################### *)
+(** ** Reformulation of the evaluation rules for heap manipulation 
+       primitive using disjoint heaps. *)
+
+Lemma eval_ref_sep : forall s1 s2 v p,
+  s2 = Fmap.single p v ->
+  Fmap.disjoint s2 s1 ->
+  eval s1 (val_ref v) (Fmap.union s2 s1) (val_loc p).
+Proof using.
+  introv -> D. forwards Dv: Fmap.indom_single p v.
+  rewrite <- Fmap.update_eq_union_single. applys* eval_ref.
+  { intros N. applys* Fmap.disjoint_inv_not_indom_both D N. }
+Qed.
+
+Lemma eval_get_sep : forall s s2 p v,
+  s = Fmap.union (Fmap.single p v) s2 ->
+  eval s (val_get (val_loc p)) s v.
+Proof using.
+  introv ->. forwards Dv: Fmap.indom_single p v.
+  applys_eq eval_get 1.
+  { applys* Fmap.indom_union_l. }
+  { rewrite* Fmap.read_union_l. rewrite* Fmap.read_single. }
+Qed.
+
+Lemma eval_set_sep : forall s1 s2 h2 p v1 v2,
+  s1 = Fmap.union (Fmap.single p v1) h2 ->
+  s2 = Fmap.union (Fmap.single p v2) h2 ->
+  Fmap.disjoint (Fmap.single p v1) h2 ->
+  eval s1 (val_set (val_loc p) v2) s2 val_unit.
+Proof using.
+  introv -> -> D. forwards Dv: Fmap.indom_single p v1.
+  applys_eq eval_set 2.
+  { applys* Fmap.indom_union_l. }
+  { rewrite* Fmap.update_union_l. fequals.
+    rewrite* Fmap.update_single. }
+Qed.
+
+Lemma eval_free_sep : forall s1 s2 v p,
+  s1 = Fmap.union (Fmap.single p v) s2 ->
+  Fmap.disjoint (Fmap.single p v) s2 ->
+  eval s1 (val_free p) s2 val_unit.
+Proof using.
+  introv -> D. forwards Dv: Fmap.indom_single p v.
+  applys_eq eval_free 2.
+  { applys* Fmap.indom_union_l. }
+  { rewrite* Fmap.remove_union_single_l.
+    intros Dl. applys Fmap.disjoint_inv_not_indom_both D Dl.
+    applys Fmap.indom_single. }
+Qed.
 
 
 (* ########################################################### *)
@@ -1017,8 +618,8 @@ Lemma hoare_conseq : forall t H' Q' H Q,
   Q' ===> Q ->
   hoare t H Q.
 Proof using.
-  introv M MH MQ HF. forwards (h'&v&R&K): M h. { himpl_fold~. }
-  exists h' v. splits~. { himpl_fold~. }
+  introv M MH MQ HF. forwards (h'&v&R&K): M h. { himpl_fold*. }
+  exists h' v. splits*. { himpl_fold*. }
 Qed.
 
 Lemma hoare_hexists : forall t (A:Type) (J:A->hprop) Q,
@@ -1031,7 +632,7 @@ Lemma hoare_hpure : forall t (P:Prop) H Q,
   hoare t (\[P] \* H) Q.
 Proof using.
   introv M. intros h (h1&h2&M1&M2&D&U). destruct M1 as (M1&HP).
-  lets E: hempty_inv HP. subst. rewrite Fmap.union_empty_l. applys~ M.
+  hnf in HP. subst. rewrite Fmap.union_empty_l. applys* M.
 Qed.
 
 Lemma hoare_val : forall v H Q,
@@ -1040,7 +641,7 @@ Lemma hoare_val : forall v H Q,
 Proof using.
   introv M. intros h K. exists h v. splits.
   { applys eval_val. }
-  { himpl_fold~. }
+  { himpl_fold*. }
 Qed.
 
 Lemma hoare_fix : forall f x t1 H Q,
@@ -1048,8 +649,8 @@ Lemma hoare_fix : forall f x t1 H Q,
   hoare (trm_fix f x t1) H Q.
 Proof using.
   introv M. intros h K. exists h __. splits.
-  { applys~ eval_fix. }
-  { himpl_fold~. }
+  { applys* eval_fix. }
+  { himpl_fold*. }
 Qed.
 
 Lemma hoare_app_fix : forall v1 v2 f x t1 H Q,
@@ -1071,7 +672,7 @@ Proof using.
   introv M1 M2 Hh.
   forwards* (h1'&v1&R1&K1): (rm M1).
   forwards* (h2'&v2&R2&K2): (rm M2).
-  exists h2' v2. splits~. { applys~ eval_let R2. }
+  exists h2' v2. splits~. { applys* eval_let R2. }
 Qed.
 
 Lemma hoare_if : forall (b:bool) t1 t2 H Q,
@@ -1089,7 +690,7 @@ Lemma hoare_add : forall H n1 n2,
 Proof using.
   intros. intros s K0. exists s (val_int (n1 + n2)). split.
   { applys eval_add. }
-  { rewrite~ hstar_hpure. }
+  { rewrite* hstar_hpure. }
 Qed.
 
 Lemma hoare_div : forall H n1 n2,
@@ -1100,7 +701,7 @@ Lemma hoare_div : forall H n1 n2,
 Proof using.
   introv N. intros s K0. exists s (val_int (Z.quot n1 n2)). split.
   { applys eval_div N. }
-  { rewrite~ hstar_hpure. }
+  { rewrite* hstar_hpure. }
 Qed.
 
 Lemma hoare_ref : forall H v,
@@ -1109,11 +710,11 @@ Lemma hoare_ref : forall H v,
     (fun r => (\exists p, \[r = val_loc p] \* p ~~> v) \* H).
 Proof using.
   intros. intros s1 K0.
-  forwards~ (p&D&N): (Fmap.single_fresh 0%nat s1 v).
+  forwards* (p&D&N): (Fmap.single_fresh 0%nat s1 v).
   exists (Fmap.union (Fmap.single p v) s1) (val_loc p). split.
-  { applys~ eval_ref_sep D. }
-  { applys~ hstar_intro.
-    { exists p. rewrite~ hstar_hpure. split~. { applys~ hsingle_intro. } } }
+  { applys* eval_ref_sep D. }
+  { applys* hstar_intro.
+    { exists p. rewrite* hstar_hpure. split~. { hnfs*. } } }
 Qed.
 
 Lemma hoare_get : forall H v p,
@@ -1123,9 +724,8 @@ Lemma hoare_get : forall H v p,
 Proof using.
   intros. intros s K0. exists s v. split.
   { destruct K0 as (s1&s2&P1&P2&D&U).
-    lets (E1&N): hsingle_inv P1. subst s1.
-    applys eval_get_sep U. }
-  { rewrite~ hstar_hpure. }
+    hnf in P1. destruct P1 as (->&N). applys eval_get_sep U. }
+  { rewrite* hstar_hpure. }
 Qed.
 
 Lemma hoare_set : forall H w p v,
@@ -1134,12 +734,11 @@ Lemma hoare_set : forall H w p v,
     (fun r => (p ~~> w) \* H).
 Proof using.
   intros. intros s1 K0.
-  destruct K0 as (h1&h2&P1&P2&D&U).
-  lets (E1&N): hsingle_inv P1.
+  destruct K0 as (h1&h2&(E1&N)&P2&D&U).
   exists (Fmap.union (Fmap.single p w) h2) val_unit. split.
   { subst h1. applys eval_set_sep U D. auto. }
-  { applys~ hstar_intro.
-    { applys~ hsingle_intro. }
+  { applys* hstar_intro.
+    { hnfs*. }
     { subst h1. applys Fmap.disjoint_single_set D. } }
 Qed.
 
@@ -1149,12 +748,18 @@ Lemma hoare_free : forall H p v,
     (fun r => H).
 Proof using.
   intros. intros s1 K0.
-  destruct K0 as (h1&h2&P1&P2&D&U).
-  lets (E1&N): hsingle_inv P1.
+  destruct K0 as (h1&h2&(E1&N)&P2&D&U).
   exists h2 val_unit. split.
   { subst h1. applys eval_free_sep U D. }
   { auto. }
 Qed.
+
+
+(** From now on, all operators have opaque definitions *)
+
+Global Opaque hempty hpure hstar hsingle hexists hforall.
+
+
 
 
 (* ########################################################### *)
@@ -1191,29 +796,16 @@ Lemma triple_conseq : forall t H' Q' H Q,
   triple t H Q.
 Proof using.
   introv M MH MQ. intros HF. applys hoare_conseq M.
-  { xchanges MH. }
-  { intros x. xchanges (MQ x). }
+  { xchange MH. xsimpl. }
+  { intros x. xchange (MQ x). xsimpl. }
 Qed.
-
-Hint Rewrite hstar_assoc hstar_hempty_l hstar_hempty_r : hstar.
-
-Ltac xmysimpl_core ::=
-  try match goal with |- _ ===> _ => intros ? end;
-  autorewrite with hstar;
-  repeat first [ apply himpl_frame_r
-               | apply himpl_frame_l 
-               | rewrite hstar_comm; apply himpl_frame_r
-               | rewrite hstar_comm; apply himpl_frame_l
-               | match goal with |- ?H ==> ?H => apply himpl_refl end
-               | match goal with |- ?H ==> ?H' => is_evar H'; apply himpl_refl end ].
-
 
 Lemma triple_frame : forall t H Q H',
   triple t H Q ->
   triple t (H \* H') (Q \*+ H').
 Proof using.
   introv M. intros HF.
-  applys hoare_conseq (M (HF \* H')); xmysimpl.
+  applys hoare_conseq (M (HF \* H')); xsimpl.
 Qed.
 
 Lemma triple_hexists : forall t (A:Type) (J:A->hprop) Q,
@@ -1232,16 +824,6 @@ Proof using.
   applys hoare_hpure. intros. applys* M.
 Qed. (* Note: can also be proved from [triple_hexists] *)
 
-Lemma triple_ramified_frame : forall H1 Q1 t H Q,
-  triple t H1 Q1 ->
-  H ==> H1 \* (Q1 \--* Q) ->
-  triple t H Q.
-Proof using.
-  introv M W. applys triple_conseq. 
-  applys triple_frame (Q1 \--* Q) M.
-  { applys W. }
-  { rewrite~ <- qwand_equiv. }
-Qed.
 
 
 (* ########################################################### *)
@@ -1251,14 +833,14 @@ Lemma triple_val : forall v H Q,
   H ==> Q v ->
   triple (trm_val v) H Q.
 Proof using.
-  introv M. intros HF. applys hoare_val. { xchanges M. }
+  introv M. intros HF. applys hoare_val. { xchange M. xsimpl. }
 Qed.
 
 Lemma triple_fix : forall f x t1 H Q,
   H ==> Q (val_fix f x t1) ->
   triple (trm_fix f x t1) H Q.
 Proof using.
-  introv M. intros HF. applys~ hoare_fix. { xchanges M. }
+  introv M. intros HF. applys* hoare_fix. { xchange M. xsimpl. }
 Qed.
 
 Lemma triple_let : forall x t1 t2 H Q Q1,
@@ -1268,7 +850,7 @@ Lemma triple_let : forall x t1 t2 H Q Q1,
 Proof using.
   introv M1 M2. intros HF. applys hoare_let.
   { applys M1. }
-  { intros v. applys hoare_conseq M2; xmysimpl. }
+  { intros v. applys hoare_conseq M2; xsimpl. }
 Qed.
 
 Lemma triple_if : forall (b:bool) t1 t2 H Q,
@@ -1295,7 +877,7 @@ Lemma triple_add : forall n1 n2,
     \[]
     (fun r => \[r = val_int (n1 + n2)]).
 Proof using.
-  intros. intros H'. applys hoare_conseq hoare_add; xmysimpl*.
+  intros. intros H'. applys hoare_conseq hoare_add; xsimpl*.
 Qed.
 
 Lemma triple_div : forall n1 n2,
@@ -1304,7 +886,7 @@ Lemma triple_div : forall n1 n2,
     \[]
     (fun r => \[r = val_int (Z.quot n1 n2)]).
 Proof using.
-  intros. intros H'. applys* hoare_conseq hoare_div; xmysimpl*.
+  intros. intros H'. applys* hoare_conseq hoare_div; xsimpl*.
 Qed.
 
 Lemma triple_ref : forall v,
@@ -1312,7 +894,7 @@ Lemma triple_ref : forall v,
     \[]
     (funloc p => p ~~> v).
 Proof using.
-  intros. intros HF. applys hoare_conseq hoare_ref; xmysimpl*.
+  intros. intros HF. applys hoare_conseq hoare_ref; xsimpl*.
 Qed.
 
 Lemma triple_get : forall v p,
@@ -1320,7 +902,7 @@ Lemma triple_get : forall v p,
     (p ~~> v)
     (fun x => \[x = v] \* (p ~~> v)).
 Proof using.
-  intros. intros HF. applys hoare_conseq hoare_get; xmysimpl*.
+  intros. intros HF. applys hoare_conseq hoare_get; xsimpl*.
 Qed.
 
 Lemma triple_set : forall w p v,
@@ -1328,7 +910,7 @@ Lemma triple_set : forall w p v,
     (p ~~> v)
     (fun _ => p ~~> w).
 Proof using.
-  intros. intros HF. applys hoare_conseq hoare_set; xmysimpl*.
+  intros. intros HF. applys hoare_conseq hoare_set; xsimpl*.
 Qed.
 
 Lemma triple_free : forall p v,
@@ -1336,6 +918,6 @@ Lemma triple_free : forall p v,
     (p ~~> v)
     (fun _ => \[]).
 Proof using.
-  intros. intros HF. applys hoare_conseq hoare_free; xmysimpl*.
+  intros. intros HF. applys hoare_conseq hoare_free; xsimpl*.
 Qed.
 
